src/lia/Lia.v
@@ -1007,7 +1007,7 @@ Transparent build_z_atom.
       destruct t0;inversion H13;clear H13;subst.
       simpl.
       rewrite Typ.i_eqb_t. simpl.
-      symmetry;apply (Zeq_is_eq_bool (Zeval_expr (interp_vmap vm') pe1) (Zeval_expr (interp_vmap vm') pe2)).
+      apply Z.eqb_eq.
     Qed.
 
     Lemma build_formula_correct :
@@ -1476,7 +1476,8 @@ Transparent build_z_atom.
      apply Zle_bool_imp_le in H2.
      apply Zle_bool_imp_le in H3.
      rewrite Typ.i_eqb_t  in H. simpl in H.
-     apply Zeq_bool_neq in H.
+     apply not_true_iff_false in H.
+     apply H. apply Z.eqb_eq.
      (*pour la beauté du geste!*) lia.
      rewrite H3 in H1; simpl in H1; elim diff_true_false; trivial.
      rewrite H2 in H0; simpl in H1; elim diff_true_false; trivial.
